Law of the Unconscious Statistician

Tristan Chaang

January 24, 2022

"This law is not a trivial result of definitions as it might at first appear, but rather must be proved." - Wikipedia

In this article I will prove the Law of the Unconscious Statistician (LOTUS).

Contents

1	Background	1
2	Preliminaries	2
3	Law of the Unconscious Statistician	2
4	The Proof on Wikipedia	3
5	Full Proof	3
6	An Example	4

1 Background

A few days ago I was writing an article titled 'On Continuous Distributions', attempting to expand as much as possible the meaning of the distributions taught in A-level's Further Mathematics Syllabus. I tried to give a proof for every detail needed to derive the pdfs of the distributions, and one of them was the definition of expectation.

I noticed the textbook wrote, the definition of E(X) is $\int_{-\infty}^{\infty} x f_X(x) dx$ whereas the definition of E(g(X)) for some function g is $\int_{-\infty}^{\infty} g(x) f_X(x) dx$. However, this got me wondering: According to the first definition, we can construct the pdf $f_{g(X)}(x)$ of g(X) and then have $E(g(X)) = \int_{-\infty}^{\infty} x f_{g(X)}(x) dx$, but this is a different form from the second definition. Unless there is a clear reason why these two forms mean the same thing, I will not accept both definitions if they can potentially clash with each other.

Assume we take the second definition instead, then $E(X) = \int_{-\infty}^{\infty} x f_X(x) dx$ follows immediately, but with this we get that $E(g(X)) = \int_{-\infty}^{\infty} x f_{g(X)}(x) dx$ again by replacing X by g(X).

Therefore, I feel there is a need to prove that the two expressions are equal. This situation is similar to how the scalar product is sometimes defined as $x_1y_1 + x_2y_2 + \cdots$, but is sometimes defined as $|X||Y|\cos\theta$. The difference is, the equivalence between these two statements is quite easy to prove.

After some attempts I couldn't manage to prove LOTUS completely because things get complicated when g(X) is not bijective. Thus I went online and see if this was well-known, and after some digging, I still couldn't find anyone giving a complete proof. However, I did find out that this relation has name, which is the Law of the Unconscious Statistician. Wikipedia gives a so-called proof, but it assumes g(x) is bijective and monotonic.

Therefore, I will try to take on the challenge to prove LOTUS completely in this article.

2 Preliminaries

1. The probability density function (pdf) $f_X(x)$ of a random variable X is the function satisfying

$$\mathcal{P}(a \le x \le b) = \int_{a}^{b} f_X(x) \, dx$$
 for all $a \le b$.

2. At every differentiable point of $\mathcal{P}(X \leq x)$, the pdf satisfies

$$f_X(x) = \frac{d}{dx} \mathcal{P}(X \le x).$$

3. The expectation of X is

$$E(X) = \int_{-\infty}^{\infty} x f_X(x) \ dx$$

4. The derivative of an invertible function g(x) is

$$\frac{dg^{-1}}{dx} = \frac{1}{g'(g^{-1}(x))}$$

3 Law of the Unconscious Statistician

Given a (Riemann integrable) function $g: \mathbb{R} \to \mathbb{R}$, the expected value of E(g(X)), if it exists, is

$$E(g(X)) = \int_{-\infty}^{\infty} g(x) f_X(x) \, dx$$

In other words,

$$\int_{-\infty}^{\infty} x f_{g(X)}(x) \, dx = \int_{-\infty}^{\infty} g(x) f_X(x) \, dx.$$

This theorem is incredibly useful because the second form of computing expectation is usually much easier to deal with, as we will see in the Example section.

4 The Proof on Wikipedia

Assume g(x) has an inverse and is strictly increasing. Then

$$E(g(X)) = \int_{-\infty}^{\infty} x f_{g(X)}(x) dx$$

$$= \int_{-\infty}^{\infty} x \left[\frac{d}{du} \mathcal{P}(g(X) \le u) \right]_{u=x} dx$$

$$= \int_{-\infty}^{\infty} x \left[\frac{d}{du} \mathcal{P}(X \le g^{-1}(u)) \right]_{u=x} dx$$

$$= \int_{-\infty}^{\infty} x \left[\frac{d}{du} F(g^{-1}(u)) \right]_{u=x} dx$$

$$= \int_{-\infty}^{\infty} x \left[F'(g^{-1}(u)) \cdot \frac{1}{g'(g^{-1}(u))} \right]_{u=x} dx$$

$$= \int_{-\infty}^{\infty} x \cdot f_X(g^{-1}(x)) \cdot \frac{1}{g'(g^{-1}(x))} dx$$

(1)

Applying the substitution $u = g^{-1}(x)$:

$$= \int_{-\infty}^{\infty} g(u) \cdot f_X(u) \ du.$$

This proof relies on the very wild assumption that g(x) has an inverse and is strictly increasing. This allows (1) to be true. Without that assumption, we have to think further.

5 Full Proof

We will dissect g(x) into sections where g is constant, strictly decreasing, or strictly increasing. Let $\cdots, I_{-1}, I_0, I_1, \cdots$ be disjoint open intervals such that $\sup I_i = \inf I_{i+1}$, and $g_i := g|_{I_i}$ is either constant or strictly monotone. Then

$$\int_{-\infty}^{\infty} x f_{g(X)}(x) dx$$

$$= \int_{-\infty}^{\infty} x \left[\frac{d}{du} \mathcal{P}(g(X) \le u) \right]_{u=x} dx$$

$$= \int_{-\infty}^{\infty} x \left[\sum_{i=-\infty}^{\infty} \frac{d}{du} \mathcal{P}(g_i(X) \le u) \right]_{u=x} dx$$
(2)

We will now analyse the value of $\frac{d}{du}\mathcal{P}(g_i(X) \leq u)$ depending on whether g_i is increasing, decreasing or constant.

If g_i is increasing and $u \in \text{Im}(g_i)$,

$$\frac{d}{du}\mathcal{P}(g_i(X) \le u) = \frac{d}{du}\mathcal{P}(X \le g_i^{-1}(u))$$

= $f_X(g_i^{-1}(u)) \cdot (g_i^{-1})'(u)$
= $\frac{f_X(g_i^{-1}(u))}{g_i'(g_i^{-1}(u))}.$

If g_i is decreasing and $u \in \text{Im}(g_i)$,

$$\frac{d}{du}\mathcal{P}(g_i(X) \le u) = \frac{d}{du}\mathcal{P}(X \ge g_i^{-1}(u))$$

= $-f_X(g_i^{-1}(u)) \cdot (g_i^{-1})'(u)$
= $-\frac{f_X(g_i^{-1}(u))}{g_i'(g_i^{-1}(u))}.$

If $u \notin \text{Im}(g_i)$ or g_i is constant, the value is either 0 or 1, thus

$$\frac{d}{du}\mathcal{P}(g_i(X) \le u) = 0.$$

Denoting $I_i = (a_i, b_i)$ and $\mu_i = \begin{cases} 1 & \text{if } g_i \text{ is increasing;} \\ -1 & \text{if } g_i \text{ is decreasing;}, \text{ the expression in (2) is} \\ 0 & \text{if } g_i \text{ constant.} \end{cases}$

$$\int_{-\infty}^{\infty} x \left[\sum_{i=-\infty}^{\infty} \frac{d}{du} \mathcal{P}(g_i(X) \le u) \right]_{u=x} dx$$
$$= \sum_{i=-\infty}^{\infty} \mu_i \int_{\min(g(a_i),g(b_i))}^{\max(g(a_i),g(b_i))} x \cdot \frac{f_X(g_i^{-1}(x))}{g_i'(g_i^{-1}(x))} dx$$

Applying the substitution $v = g_i^{-1}(x)$ and noting how μ_i swaps the bounds, the above is equal to

$$\sum_{i=-\infty}^{\infty} \int_{a_i}^{b_i} g_i(v) \cdot f_X(v) \, dv = \int_{-\infty}^{\infty} g(x) \cdot f_X(x) \, dx,$$

as desired.

6 An Example

Assume $g(x) = x^2$ and $f_X(x) = \frac{1}{100}$ for $-20 \le x \le 80$ and $f_X(x) = 0$ otherwose. Then

$$f_{X^2}(x) = \frac{d}{dx} \mathcal{P}(X^2 \le x)$$

г	
L	
∟	

If $x \le 0$, then $f_{X^2}(x) = 0$. If x > 0,

$$\frac{d}{dx}\mathcal{P}(X^2 \le x)$$

$$= \frac{d}{dx}\mathcal{P}\left(-\sqrt{x} \le X \le \sqrt{x}\right)$$

$$= \frac{d}{dx}\left(\mathcal{P}\left(X \le \sqrt{x}\right) - \mathcal{P}\left(X \le -\sqrt{x}\right)\right)$$

$$= f_X(\sqrt{x}) \cdot \frac{1}{2\sqrt{x}} - f_X(-\sqrt{x}) \cdot \left(-\frac{1}{2\sqrt{x}}\right)$$

$$= \begin{cases} \frac{1}{100\sqrt{x}} & \text{if } 0 < x \le 400; \\ \frac{1}{200\sqrt{x}} & \text{if } 400 < x \le 6400; \\ 0 & \text{otherwise.} \end{cases}$$

We have two ways to compute $E(X^2)$. One,

$$E(X^2) = \int_0^{400} x \cdot \frac{1}{100\sqrt{x}} \, dx + \int_{400}^{6400} x \cdot \frac{1}{200\sqrt{x}} \, dx$$
$$= \frac{1}{150} \cdot 400^{3/2} + \frac{1}{300} \cdot 6400^{3/2} - \frac{1}{300} \cdot 400^{3/2}$$
$$= \frac{5200}{3}.$$

Two,

$$E(X^2) = \int_{-20}^{80} x^2 \cdot \frac{1}{100} dx$$

= $\frac{1}{100} \left(\frac{80^3}{3} - \frac{(-20)^3}{3} \right)$
= $\frac{5200}{3}$.

We see that the answers are consistent. This is exactly what we were looking for.

References

- [1] Law of the Unconscious Statistician https://en.wikipedia.org/wiki/Law_of_the_unconscious_statistician
- [2] On Continuous Distributions https://tristanchaang.github.io/2022/01/07/on-continuous-distributions.html